<?xml version="1.0"?>
<rdf:RDF xmlns="https://w3id.org/citydata/part3/v1/"
     xml:base="https://w3id.org/citydata/part3/v1/"
     xmlns:cc="http://creativecommons.org/ns#"
     xmlns:dcterms="http://purl.org/dc/terms/"
     xmlns:owl="http://www.w3.org/2002/07/owl#"
     xmlns:rdf="http://www.w3.org/1999/02/22-rdf-syntax-ns#"
     xmlns:rdfs="http://www.w3.org/2000/01/rdf-schema#"
     xmlns:skos="http://www.w3.org/2004/02/skos/core#"
     xmlns:vann="http://purl.org/vocab/vann/"
     xmlns:xml="http://www.w3.org/XML/1998/namespace"
     xmlns:xsd="http://www.w3.org/2001/XMLSchema#">
    <owl:Ontology rdf:about="https://w3id.org/citydata/part3/v1/Core/">
    	<!-- Identity -->
    	<dcterms:title>Information technology - City data model - Part 3: Service level concepts - Core</dcterms:title>
    	<skos:definition>This ontology specifies the service-level concepts defined for the transport service of the city data model.</skos:definition>
    	<vann:preferredNamespaceUri>https://w3id.org/citydata/part3/v1/</vann:preferredNamespaceUri>
    	<vann:preferredNamespacePrefix>cdm3</vann:preferredNamespacePrefix>
    		
    	<!-- Provenance -->
        <dcterms:creator>Megan Katsumi</dcterms:creator>
        <dcterms:creator>Mark Fox</dcterms:creator>
    	<dcterms:creator>Kenneth Vaughn</dcterms:creator>
        <!-- This release -->
		<dcterms:modified rdf:datatype="http://www.w3.org/2001/XMLSchema#date">2026-02-12</dcterms:modified> 
        <owl:versionInfo>1.0.0</owl:versionInfo>
        <owl:versionIRI rdf:resource="https://w3id.org/citydata/part3/v1/Core/r0.0"/>
   
        <!-- License -->
        <cc:license>http://creativecommons.org/licenses/by/4.0/</cc:license>
        
        <!-- Imports -->
        <owl:imports rdf:resource="https://w3id.org/citydata/part2/v1/Core/"/> 

    </owl:Ontology>

    <!-- 
    ///////////////////////////////////////////////////////////////////////////////////////
    //
    // Object Properties
    //
    ///////////////////////////////////////////////////////////////////////////////////////
     -->


    <!-- https://w3id.org/citydata/part3/v1/ITSObjectProperty -->

    <owl:ObjectProperty rdf:about="https://w3id.org/citydata/part3/v1/ITSObjectProperty">
        <rdfs:subPropertyOf rdf:resource="https://w3id.org/citydata/part1/v1/CdmObjectProperty"/>
        <skos:definition>Added for organizational purposes, to identify all object properties defined for the transport service of the City Data Model.</skos:definition>
    </owl:ObjectProperty>


    <!-- 
    ///////////////////////////////////////////////////////////////////////////////////////
    //
    // Data properties
    //
    ///////////////////////////////////////////////////////////////////////////////////////
     -->


    <!-- https://w3id.org/citydata/part3/v1/FoundationalCdmDataProperty -->

    <owl:DatatypeProperty rdf:about="https://w3id.org/citydata/part3/v1/ITSDataProperty">
        <rdfs:subPropertyOf rdf:resource="https://w3id.org/citydata/part1/v1/CdmDataProperty"/>
        <skos:definition>Added for organizational purposes, to identify all data properties defined for the transport service of the City Data Model.</skos:definition>
    </owl:DatatypeProperty>

     <!-- 
    ///////////////////////////////////////////////////////////////////////////////////////
    //
    // Classes
    //
    ///////////////////////////////////////////////////////////////////////////////////////
     -->

    <!-- https://w3id.org/citydata/part3/v1/ITSThing -->

    <owl:Class rdf:about="https://w3id.org/citydata/part3/v1/ITSThing">
        <skos:definition>Added for organizational purposes, to identify all classes defined for the transport service of the City Data Model.</skos:definition>
        <rdfs:subClassOf rdf:resource="https://w3id.org/citydata/part1/v1/CdmThing"/>
    </owl:Class>


</rdf:RDF>    