<?xml version="1.0"?>
<rdf:RDF xmlns="https://w3id.org/citydata/part3/v1/"
     xml:base="https://w3id.org/citydata/part3/v1/"
     xmlns:cc="http://creativecommons.org/ns#"
     xmlns:dash="http://datashapes.org/dash#"
     xmlns:dcterms="http://purl.org/dc/terms/"
     xmlns:owl="http://www.w3.org/2002/07/owl#"
     xmlns:rdf="http://www.w3.org/1999/02/22-rdf-syntax-ns#"
     xmlns:rdfs="http://www.w3.org/2000/01/rdf-schema#"
     xmlns:skos="http://www.w3.org/2004/02/skos/core#"
     xmlns:vann="http://purl.org/vocab/vann/"
     xmlns:xml="http://www.w3.org/XML/1998/namespace"
     xmlns:xsd="http://www.w3.org/2001/XMLSchema#"
     xmlns:geo="https://www.opengis.net/ont/geosparql#"
     xmlns:time="https://www.w3.org/2006/time#"
     xmlns:cdm1="https://w3id.org/citydata/part1/v1/"
     xmlns:cdm2="https://w3id.org/citydata/part2/v1/">

    <owl:Ontology rdf:about="https://w3id.org/citydata/part3/v1/PublicTransportSystemPattern/">
    	<!-- Identity -->
    	<dcterms:title>Information technology - City data model - Part 3: Service-level concepts for transport - Transport network pattern</dcterms:title>
    	<skos:definition>This ontology specifies the service-level concepts for transport in the city data model.</skos:definition>
    	<vann:preferredNamespaceUri>https://w3id.org/citydata/part3/v1/</vann:preferredNamespaceUri>
    	<vann:preferredNamespacePrefix>cdm3</vann:preferredNamespacePrefix>
    		
    	<!-- Provenance -->
    	<dcterms:creator>Kenneth Vaughn</dcterms:creator>
        <dcterms:creator>Tom Lusco</dcterms:creator>
        <dcterms:creator>Megan Katsumi</dcterms:creator>
        <dcterms:creator>Mark Fox</dcterms:creator>
        <!-- Prior release - None -->
        <!-- This release -->
		<dcterms:modified rdf:datatype="http://www.w3.org/2001/XMLSchema#date">2026-02-13</dcterms:modified> <!-- Date of this ontology file -->
        <owl:versionInfo>1.0.0</owl:versionInfo>
        <owl:versionIRI rdf:resource="https://w3id.org/citydata/part3/v1/PublicTransportSystemPattern/r0.0"/>
        
        <!-- License -->
        <cc:license>http://creativecommons.org/licenses/by/4.0/</cc:license>
        
        <!-- Imports -->
        <owl:imports rdf:resource="https://w3id.org/citydata/part3/v1/TransportNetworkPattern/"/>
    </owl:Ontology>
    

    <!-- 
    ///////////////////////////////////////////////////////////////////////////////////////
    //
    // Object Properties
    //
    ///////////////////////////////////////////////////////////////////////////////////////
     -->


     <!-- https://w3id.org/citydata/part3/v1/PublicTransportSystemObjectProperty -->

    <owl:ObjectProperty rdf:about="https://w3id.org/citydata/part3/v1/PublicTransportSystemObjectProperty">
        <skos:definition>Added for organizational purposes, to identify all object properties defined in the Public Transport System Pattern.</skos:definition>
        <rdfs:subPropertyOf rdf:resource="https://w3id.org/citydata/part3/v1/ITSObjectProperty"/>
    </owl:ObjectProperty>
    

    <!-- https://w3id.org/citydata/part3/v1/direction -->

    <owl:ObjectProperty rdf:about="https://w3id.org/citydata/part3/v1/direction">
        <dcterms:description>A code representing the direction of operation.</dcterms:description>
        <rdfs:subPropertyOf rdf:resource="https://w3id.org/citydata/part3/v1/PublicTransportSystemObjectProperty"/>
        <rdfs:range rdf:resource="https://w3id.org/citydata/part2/v1/Code"/>
    </owl:ObjectProperty>
    

    <!-- https://w3id.org/citydata/part3/v1/routePoint -->

    <owl:ObjectProperty rdf:about="https://w3id.org/citydata/part3/v1/routePoint">
        <dcterms:description>A TransportNode that represents a point of interest along a PublicTransportRoute.</dcterms:description>
        <rdfs:subPropertyOf rdf:resource="https://w3id.org/citydata/part3/v1/PublicTransportSystemObjectProperty"/>
        <rdfs:range rdf:resource="https://w3id.org/citydata/part3/v1/RoutePoint"/>
    </owl:ObjectProperty>
    

    <!-- https://w3id.org/citydata/part3/v1/routePointType -->

    <owl:ObjectProperty rdf:about="https://w3id.org/citydata/part3/v1/routePointType">
        <dcterms:description>An indication of the type of route point.</dcterms:description>
        <rdfs:subPropertyOf rdf:resource="https://w3id.org/citydata/part3/v1/PublicTransportSystemObjectProperty"/>
        <rdfs:range rdf:resource="https://w3id.org/citydata/part2/v1/Code"/>
    </owl:ObjectProperty>
    

    <!-- https://w3id.org/citydata/part3/v1/routePoints -->

    <owl:ObjectProperty rdf:about="https://w3id.org/citydata/part3/v1/routePoints">
        <dcterms:description>An ordered series of route points along a PublicTransportRoute.</dcterms:description>
        <rdfs:subPropertyOf rdf:resource="https://w3id.org/citydata/part3/v1/PublicTransportSystemObjectProperty"/>
        <rdfs:range rdf:resource="https://w3id.org/citydata/part3/v1/PointOnRoute"/>
    </owl:ObjectProperty>
    

    <!-- 
    ///////////////////////////////////////////////////////////////////////////////////////
    //
    // Data properties
    //
    ///////////////////////////////////////////////////////////////////////////////////////
     -->


    <!-- https://w3id.org/citydata/part3/v1/PublicTransportSystemDataProperty -->

    <owl:DatatypeProperty rdf:about="https://w3id.org/citydata/part3/v1/PublicTransportSystemDataProperty">
        <skos:definition>Added for organizational purposes, to identify all data properties defined in the Public Transport System Pattern.</skos:definition>
        <rdfs:subPropertyOf rdf:resource="https://w3id.org/citydata/part3/v1/ITSDataProperty"/>
    </owl:DatatypeProperty>
    

    <!-- https://w3id.org/citydata/part3/v1/index -->

    <owl:DatatypeProperty rdf:about="https://w3id.org/citydata/part3/v1/index">
        <dcterms:description>integer value that indicates the order of the item in a list</dcterms:description>
        <rdfs:subPropertyOf rdf:resource="https://w3id.org/citydata/part3/v1/PublicTransportSystemDataProperty"/>
        <rdfs:range rdf:resource="http://www.w3.org/2001/XMLSchema#integer"/>
    </owl:DatatypeProperty>
    

    <!-- https://w3id.org/citydata/part3/v1/isBorderCrossing -->

    <owl:DatatypeProperty rdf:about="https://w3id.org/citydata/part3/v1/isBorderCrossing">
        <dcterms:description>A boolean value that indicates whether the node serves as a border crossing.</dcterms:description>
        <rdfs:subPropertyOf rdf:resource="https://w3id.org/citydata/part3/v1/PublicTransportSystemDataProperty"/>
        <rdfs:range rdf:resource="http://www.w3.org/2001/XMLSchema#boolean"/>
    </owl:DatatypeProperty>
    

    <!-- https://w3id.org/citydata/part3/v1/isViaPoint -->

    <owl:DatatypeProperty rdf:about="https://w3id.org/citydata/part3/v1/isViaPoint">
        <dcterms:description>A boolean value that indicates whether the node is referenced as a part-way point on a route.</dcterms:description>
        <rdfs:subPropertyOf rdf:resource="https://w3id.org/citydata/part3/v1/PublicTransportSystemDataProperty"/>
        <rdfs:range rdf:resource="http://www.w3.org/2001/XMLSchema#boolean"/>
    </owl:DatatypeProperty>
    

    <!-- 
    ///////////////////////////////////////////////////////////////////////////////////////
    //
    // Classes
    //
    ///////////////////////////////////////////////////////////////////////////////////////
     -->


    <!-- https://w3id.org/citydata/part3/v1/PublicTransportSystemThing -->

    <owl:Class rdf:about="https://w3id.org/citydata/part3/v1/PublicTransportSystemThing">
        <skos:definition>Added for organizational purposes, to identify classes defined in the Public Transport System Pattern ontology.</skos:definition>
        <rdfs:subClassOf rdf:resource="https://w3id.org/citydata/part3/v1/ITSThing"/>
    </owl:Class>
    

    <!-- https://w3id.org/citydata/part3/v1/PublicTransportElement -->

    <owl:Class rdf:about="https://w3id.org/citydata/part3/v1/PublicTransportElement">
        <skos:definition>A PublicTransportElement represents any element of a public transport system. It can be a part of another PublicTransportElement and can be decomposed into smaller PublicTransportElement.</skos:definition>
        <rdfs:subClassOf rdf:resource="https://w3id.org/citydata/part3/v1/PublicTransportSystemThing"/>
        <rdfs:subClassOf rdf:resource="https://w3id.org/citydata/part2/v1/InfrastructureElement"/>
    </owl:Class>
    

     <!-- https://w3id.org/citydata/part3/v1/GroupOfLines -->

    <owl:Class rdf:about="https://w3id.org/citydata/part3/v1/GroupOfLines">
        <dcterms:description>A GroupOfLines is a logical grouping of PublicTransportLines for any useful purpose.</dcterms:description>
        <rdfs:subClassOf rdf:resource="https://w3id.org/citydata/part3/v1/PublicTransportElement"/>
        <rdfs:subClassOf>
            <owl:Restriction>
                <owl:onProperty rdf:resource="https://w3id.org/citydata/part1/v1/hasProperPart"/>
                <owl:allValuesFrom rdf:resource="https://w3id.org/citydata/part3/v1/PublicTransportLine"/>
            </owl:Restriction>
        </rdfs:subClassOf>
        <rdfs:subClassOf>
            <owl:Restriction>
                <owl:onProperty rdf:resource="https://w3id.org/citydata/part1/v1/properPartOf"/>
                <owl:allValuesFrom rdf:resource="https://w3id.org/citydata/part3/v1/PublicTransportSystem"/>
            </owl:Restriction>
        </rdfs:subClassOf>
        <rdfs:subClassOf>
            <owl:Restriction>
                <owl:onProperty rdf:resource="https://w3id.org/citydata/part1/v1/hasProperPart"/>
                <owl:minQualifiedCardinality rdf:datatype="http://www.w3.org/2001/XMLSchema#nonNegativeInteger">1</owl:minQualifiedCardinality>
                <owl:onClass rdf:resource="https://w3id.org/citydata/part3/v1/PublicTransportLine"/>
            </owl:Restriction>
        </rdfs:subClassOf>
    </owl:Class>
    

    <!-- https://w3id.org/citydata/part3/v1/PointOnRoute -->

    <owl:Class rdf:about="https://w3id.org/citydata/part3/v1/PointOnRoute">
        <dcterms:description>A PointOnRoute represents an ordered RoutePoint for a PublicTransportRoute.</dcterms:description>
        <rdfs:subClassOf rdf:resource="https://w3id.org/citydata/part3/v1/PublicTransportElement"/>
        <rdfs:subClassOf>
            <owl:Restriction>
                <owl:onProperty rdf:resource="https://w3id.org/citydata/part3/v1/routePointType"/>
                <owl:allValuesFrom rdf:resource="https://w3id.org/citydata/part2/v1/Code"/>
            </owl:Restriction>
        </rdfs:subClassOf>
        <rdfs:subClassOf>
            <owl:Restriction>
                <owl:onProperty rdf:resource="https://w3id.org/citydata/part3/v1/routePoint"/>
                <owl:qualifiedCardinality rdf:datatype="http://www.w3.org/2001/XMLSchema#nonNegativeInteger">1</owl:qualifiedCardinality>
                <owl:onClass rdf:resource="https://w3id.org/citydata/part3/v1/RoutePoint"/>
            </owl:Restriction>
        </rdfs:subClassOf>
        <rdfs:subClassOf>
            <owl:Restriction>
                <owl:onProperty rdf:resource="https://w3id.org/citydata/part3/v1/index"/>
                <owl:qualifiedCardinality rdf:datatype="http://www.w3.org/2001/XMLSchema#nonNegativeInteger">1</owl:qualifiedCardinality>
                <owl:onDataRange rdf:resource="http://www.w3.org/2001/XMLSchema#integer"/>
            </owl:Restriction>
        </rdfs:subClassOf>
    </owl:Class>
    

    <!-- https://w3id.org/citydata/part3/v1/PublicTransportLine -->

    <owl:Class rdf:about="https://w3id.org/citydata/part3/v1/PublicTransportLine">
        <dcterms:description>A PublicTransportLine is one or more routes used by public transport vehicles to transport passengers to and from designated locations.</dcterms:description>
        <rdfs:subClassOf rdf:resource="https://w3id.org/citydata/part3/v1/PublicTransportElement"/>
        <rdfs:subClassOf>
            <owl:Restriction>
                <owl:onProperty rdf:resource="https://w3id.org/citydata/part1/v1/properPartOf"/>
                <owl:allValuesFrom>
                    <owl:Class>
                        <owl:unionOf rdf:parseType="Collection">
                            <rdf:Description rdf:about="https://w3id.org/citydata/part3/v1/GroupOfLines"/>
                            <rdf:Description rdf:about="https://w3id.org/citydata/part3/v1/PublicTransportSystem"/>
                        </owl:unionOf>
                    </owl:Class>
                </owl:allValuesFrom>
            </owl:Restriction>
        </rdfs:subClassOf>
        <rdfs:subClassOf>
            <owl:Restriction>
                <owl:onProperty rdf:resource="https://w3id.org/citydata/part1/v1/hasProperPart"/>
                <owl:allValuesFrom rdf:resource="https://w3id.org/citydata/part3/v1/PublicTransportRoute"/>
            </owl:Restriction>
        </rdfs:subClassOf>
        <rdfs:subClassOf>
            <owl:Restriction>
                <owl:onProperty rdf:resource="https://w3id.org/citydata/part1/v1/hasProperPart"/>
                <owl:minQualifiedCardinality rdf:datatype="http://www.w3.org/2001/XMLSchema#nonNegativeInteger">1</owl:minQualifiedCardinality>
                <owl:onClass rdf:resource="https://w3id.org/citydata/part3/v1/PublicTransportRoute"/>
            </owl:Restriction>
        </rdfs:subClassOf>
        <rdfs:subClassOf>
            <owl:Restriction>
                <owl:onProperty rdf:resource="https://w3id.org/citydata/part3/v1/allowedDirections"/>
                <owl:minQualifiedCardinality rdf:datatype="http://www.w3.org/2001/XMLSchema#nonNegativeInteger">1</owl:minQualifiedCardinality>
                <owl:onClass rdf:resource="https://w3id.org/citydata/part2/v1/Code"/>
            </owl:Restriction>
        </rdfs:subClassOf>
    </owl:Class>
    


    <!-- https://w3id.org/citydata/part3/v1/PublicTransportRoute -->

    <owl:Class rdf:about="https://w3id.org/citydata/part3/v1/PublicTransportRoute">
        <dcterms:description>A PublicTransportRoute represents one specific path used by a public transport vehicle to transport passengers to and from designated locations.</dcterms:description>
        <skos:note>For example, a PublicTransportLine might use an alternate PublicTransportRoute to reach its next stop during periods of congestion.</skos:note>
        <rdfs:subClassOf rdf:resource="https://w3id.org/citydata/part3/v1/PublicTransportElement"/>
        <rdfs:subClassOf>
            <owl:Restriction>
                <owl:onProperty rdf:resource="https://w3id.org/citydata/part1/v1/properPartOf"/>
                <owl:allValuesFrom rdf:resource="https://w3id.org/citydata/part3/v1/PublicTransportLine"/>
            </owl:Restriction>
        </rdfs:subClassOf>
        <rdfs:subClassOf>
            <owl:Restriction>
                <owl:onProperty rdf:resource="https://w3id.org/citydata/part1/v1/properPartOf"/>
                <owl:minQualifiedCardinality rdf:datatype="http://www.w3.org/2001/XMLSchema#nonNegativeInteger">1</owl:minQualifiedCardinality>
                <owl:onClass rdf:resource="https://w3id.org/citydata/part3/v1/PublicTransportLine"/>
            </owl:Restriction>
        </rdfs:subClassOf>
        <rdfs:subClassOf>
            <owl:Restriction>
                <owl:onProperty rdf:resource="https://w3id.org/citydata/part3/v1/direction"/>
                <owl:minQualifiedCardinality rdf:datatype="http://www.w3.org/2001/XMLSchema#nonNegativeInteger">1</owl:minQualifiedCardinality>
                <owl:onClass rdf:resource="https://w3id.org/citydata/part2/v1/Code"/>
            </owl:Restriction>
        </rdfs:subClassOf>
        <rdfs:subClassOf>
            <owl:Restriction>
                <owl:onProperty rdf:resource="https://w3id.org/citydata/part3/v1/routePoints"/>
                <owl:minQualifiedCardinality rdf:datatype="http://www.w3.org/2001/XMLSchema#nonNegativeInteger">2</owl:minQualifiedCardinality>
                <owl:onClass rdf:resource="https://w3id.org/citydata/part3/v1/PointOnRoute"/>
            </owl:Restriction>
        </rdfs:subClassOf>
    </owl:Class>
    

    <!-- https://w3id.org/citydata/part3/v1/PublicTransportSystem -->

    <owl:Class rdf:about="https://w3id.org/citydata/part3/v1/PublicTransportSystem">
        <dcterms:description>A PublicTransportSystem provides transport services to members of the public.</dcterms:description>
        <rdfs:subClassOf rdf:resource="https://w3id.org/citydata/part3/v1/PublicTransportElement"/>
        <rdfs:subClassOf>
            <owl:Restriction>
                <owl:onProperty rdf:resource="https://w3id.org/citydata/part1/v1/hasProperPart"/>
                <owl:allValuesFrom>
                    <owl:Class>
                        <owl:unionOf rdf:parseType="Collection">
                            <rdf:Description rdf:about="https://w3id.org/citydata/part3/v1/GroupOfLines"/>
                            <rdf:Description rdf:about="https://w3id.org/citydata/part3/v1/PublicTransportLine"/>
                        </owl:unionOf>
                    </owl:Class>
                </owl:allValuesFrom>
            </owl:Restriction>
        </rdfs:subClassOf>
    </owl:Class>
    

    <!-- https://w3id.org/citydata/part3/v1/RoutePoint -->

    <owl:Class rdf:about="https://w3id.org/citydata/part3/v1/RoutePoint">
        <dcterms:description>A RoutePoint represents a point of interest along a PublicTransportRoute.</dcterms:description>
        <rdfs:subClassOf rdf:resource="https://w3id.org/citydata/part3/v1/PublicTransportElement"/>
        <rdfs:subClassOf rdf:resource="https://w3id.org/citydata/part3/v1/TransportNode"/>
        <rdfs:subClassOf>
            <owl:Restriction>
                <owl:onProperty rdf:resource="https://w3id.org/citydata/part3/v1/isBorderCrossing"/>
                <owl:qualifiedCardinality rdf:datatype="http://www.w3.org/2001/XMLSchema#nonNegativeInteger">1</owl:qualifiedCardinality>
                <owl:onDataRange rdf:resource="http://www.w3.org/2001/XMLSchema#boolean"/>
            </owl:Restriction>
        </rdfs:subClassOf>
        <rdfs:subClassOf>
            <owl:Restriction>
                <owl:onProperty rdf:resource="https://w3id.org/citydata/part3/v1/isViaPoint"/>
                <owl:maxQualifiedCardinality rdf:datatype="http://www.w3.org/2001/XMLSchema#nonNegativeInteger">1</owl:maxQualifiedCardinality>
                <owl:onDataRange rdf:resource="http://www.w3.org/2001/XMLSchema#boolean"/>
            </owl:Restriction>
        </rdfs:subClassOf>
    </owl:Class>
    
</rdf:RDF>
