<?xml version="1.0"?>
<rdf:RDF xmlns="https://w3id.org/citydata/part3/v1/"
     xml:base="https://w3id.org/citydata/part3/v1/"
     xmlns:cc="http://creativecommons.org/ns#"
     xmlns:dash="http://datashapes.org/dash#"
     xmlns:dcterms="http://purl.org/dc/terms/"
     xmlns:owl="http://www.w3.org/2002/07/owl#"
     xmlns:rdf="http://www.w3.org/1999/02/22-rdf-syntax-ns#"
     xmlns:rdfs="http://www.w3.org/2000/01/rdf-schema#"
     xmlns:skos="http://www.w3.org/2004/02/skos/core#"
     xmlns:vann="http://purl.org/vocab/vann/"
     xmlns:xml="http://www.w3.org/XML/1998/namespace"
     xmlns:xsd="http://www.w3.org/2001/XMLSchema#"
     xmlns:geo="https://www.opengis.net/ont/geosparql#"
     xmlns:time="https://www.w3.org/2006/time#"
     xmlns:cdm1="https://w3id.org/citydata/part1/v1/"
     xmlns:cdm2="https://w3id.org/citydata/part2/v1/">

    <owl:Ontology rdf:about="https://w3id.org/citydata/part3/v1/TravelCorridorPattern/">
    	<!-- Identity -->
    	<dcterms:title>Information technology - City data model - Part 3: Service-level concepts for transport - Travel corridor pattern</dcterms:title>
    	<skos:definition>This ontology specifies the service-level concepts for the travel corridor pattern in the city data model.</skos:definition>
    	<vann:preferredNamespaceUri>https://w3id.org/citydata/part3/v1/</vann:preferredNamespaceUri>
    	<vann:preferredNamespacePrefix>cdm3</vann:preferredNamespacePrefix>
    		
    	<!-- Provenance -->
    	<dcterms:creator>Kenneth Vaughn</dcterms:creator>
        <dcterms:creator>Tom Lusco</dcterms:creator>
        <dcterms:creator>Megan Katsumi</dcterms:creator>
        <dcterms:creator>Mark Fox</dcterms:creator>
        <!-- Prior release - None -->
        <!-- This release -->
		<dcterms:modified rdf:datatype="http://www.w3.org/2001/XMLSchema#date">2026-02-13</dcterms:modified> 
        <owl:versionInfo>1.0.0</owl:versionInfo>
        <owl:versionIRI rdf:resource="https://w3id.org/citydata/part3/v1/TravelCorridorPattern/r0.0"/>
        
        <!-- License -->
        <cc:license>http://creativecommons.org/licenses/by/4.0/</cc:license>
        
        <!-- Imports -->
         <owl:imports rdf:resource="https://w3id.org/citydata/part3/v1/TransportNetworkPattern/"/>
    </owl:Ontology>
    

    <!-- 
    ///////////////////////////////////////////////////////////////////////////////////////
    //
    // Object Properties
    //
    ///////////////////////////////////////////////////////////////////////////////////////
     -->


    <!-- https://w3id.org/citydata/part3/v1/TravelCorridorObjectProperty -->

    <owl:ObjectProperty rdf:about="https://w3id.org/citydata/part3/v1/TravelCorridorObjectProperty">
        <skos:definition>Added for organizational purposes, to identify all object properties defined in the Travel Corridor Pattern.</skos:definition>
        <rdfs:subPropertyOf rdf:resource="https://w3id.org/citydata/part3/v1/ITSObjectProperty"/>
    </owl:ObjectProperty>
    

    <!-- https://w3id.org/citydata/part3/v1/corridorElement -->

    <owl:ObjectProperty rdf:about="https://w3id.org/citydata/part3/v1/corridorElement">
        <dcterms:description>An NetworkElement that is considered to be part of the larger transport corridor.</dcterms:description>
        <rdfs:subPropertyOf rdf:resource="https://w3id.org/citydata/part3/v1/TravelCorridorObjectProperty"/>
        <rdfs:range rdf:resource="https://w3id.org/citydata/part3/v1/TravelledWaySegment"/>
    </owl:ObjectProperty>
    

    <!-- 
    ///////////////////////////////////////////////////////////////////////////////////////
    //
    // Classes
    //
    ///////////////////////////////////////////////////////////////////////////////////////
     -->


    <!-- https://w3id.org/citydata/part3/v1/TravelCorridorThing -->

    <owl:ObjectProperty rdf:about="https://w3id.org/citydata/part3/v1/TravelCorridorThing">
        <skos:definition>Added for organizational purposes, to identify all classes defined in the Travel Corridor Pattern.</skos:definition>
        <rdfs:subPropertyOf rdf:resource="https://w3id.org/citydata/part3/v1/ITSThing"/>
    </owl:ObjectProperty>
    

     <!-- https://w3id.org/citydata/part3/v1/TravelCorridor -->

    <owl:Class rdf:about="https://w3id.org/citydata/part3/v1/TravelCorridor">
        <dcterms:description>A TravelCorridor is a type of TravelledWay that is made up of TravelCorridorLinks.</dcterms:description>
        <skos:note>The extent of a TravelCorridor is defined by the extent of the path that shares the designator assigned to the TravelCorridor.</skos:note>
        <rdfs:subClassOf rdf:resource="https://w3id.org/citydata/part3/v1/TravelCorridorThing"/>
        <rdfs:subClassOf rdf:resource="https://w3id.org/citydata/part3/v1/TravelledWay"/>
        <rdfs:subClassOf>
            <owl:Restriction>
                <owl:onProperty rdf:resource="https://w3id.org/citydata/part1/v1/hasProperPart"/>
                <owl:allValuesFrom rdf:resource="https://w3id.org/citydata/part3/v1/TravelCorridorLink"/>
            </owl:Restriction>
        </rdfs:subClassOf>
        <rdfs:subClassOf>
            <owl:Restriction>
                <owl:onProperty rdf:resource="https://w3id.org/citydata/part1/v1/hasProperPart"/>
                <owl:minQualifiedCardinality rdf:datatype="http://www.w3.org/2001/XMLSchema#nonNegativeInteger">1</owl:minQualifiedCardinality>
                <owl:onClass rdf:resource="https://w3id.org/citydata/part3/v1/TravelCorridorLink"/>
            </owl:Restriction>
        </rdfs:subClassOf>
    </owl:Class>
    


    <!-- https://w3id.org/citydata/part3/v1/TravelCorridorLink -->

    <owl:Class rdf:about="https://w3id.org/citydata/part3/v1/TravelCorridorLink">
        <dcterms:description>A TravelCorridorLink is a type of TravelledWayLink that is made up of TravelCorridorSegments.</dcterms:description>
        <rdfs:subClassOf rdf:resource="https://w3id.org/citydata/part3/v1/TravelCorridorThing"/>
        <rdfs:subClassOf rdf:resource="https://w3id.org/citydata/part3/v1/TravelledWayLink"/>
        <rdfs:subClassOf>
            <owl:Restriction>
                <owl:onProperty rdf:resource="https://w3id.org/citydata/part1/v1/hasProperPart"/>
                <owl:allValuesFrom rdf:resource="https://w3id.org/citydata/part3/v1/TravelCorridorSegment"/>
            </owl:Restriction>
        </rdfs:subClassOf>
        <rdfs:subClassOf>
            <owl:Restriction>
                <owl:onProperty rdf:resource="https://w3id.org/citydata/part1/v1/hasProperPart"/>
                <owl:allValuesFrom rdf:resource="https://w3id.org/citydata/part3/v1/TravelCorridor"/>
            </owl:Restriction>
        </rdfs:subClassOf>
        <rdfs:subClassOf>
            <owl:Restriction>
                <owl:onProperty rdf:resource="https://w3id.org/citydata/part1/v1/hasProperPart"/>
                <owl:minQualifiedCardinality rdf:datatype="http://www.w3.org/2001/XMLSchema#nonNegativeInteger">1</owl:minQualifiedCardinality>
                <owl:onClass rdf:resource="https://w3id.org/citydata/part3/v1/TravelCorridorSegment"/>
            </owl:Restriction>
        </rdfs:subClassOf>
    </owl:Class>
    

    <!-- https://w3id.org/citydata/part3/v1/TravelCorridorSegment -->

    <owl:Class rdf:about="https://w3id.org/citydata/part3/v1/TravelCorridorSegment">
        <dcterms:description>A TravelCorridorSegment is a type of TravelledWaySegment that logically groups multiple TravelledWaySegments together as being co-located or side-by-side.</dcterms:description>
        <rdfs:subClassOf rdf:resource="https://w3id.org/citydata/part3/v1/TravelCorridorThing"/>
        <rdfs:subClassOf rdf:resource="https://w3id.org/citydata/part3/v1/TravelledWaySegment"/>
        <rdfs:subClassOf>
            <owl:Restriction>
                <owl:onProperty rdf:resource="https://w3id.org/citydata/part1/v1/properPartOf"/>
                <owl:allValuesFrom rdf:resource="https://w3id.org/citydata/part3/v1/TravelCorridorLink"/>
            </owl:Restriction>
        </rdfs:subClassOf>
        <rdfs:subClassOf>
            <owl:Restriction>
                <owl:onProperty rdf:resource="https://w3id.org/citydata/part3/v1/corridorElement"/>
                <owl:minQualifiedCardinality rdf:datatype="http://www.w3.org/2001/XMLSchema#nonNegativeInteger">1</owl:minQualifiedCardinality>
                <owl:onClass rdf:resource="https://w3id.org/citydata/part3/v1/TravelledWaySegment"/>
            </owl:Restriction>
        </rdfs:subClassOf>
    </owl:Class>
    

</rdf:RDF>
